

Module – 6.5

# FROM GAUSS TO KALMAN: SEQUENTIAL, LINEAR MINIMUM VARIANCE ESTIMATION

S. Lakshmivarahan

*School of Computer Science*

*University of Oklahoma*

*Norman, Ok – 73069, USA*

[varahan@ou.edu](mailto:varahan@ou.edu)

# LINEAR MINIMUM VARIANCE ESTIMATE

---

- Similar to Gauss-Markov theorem in Chapter 14 (LLD (2006))
- $z = Hx + v$
- Assumptions:
  - $E(v) = 0$ ,  $COV(v) = \Sigma_v$  – SPD
  - $E(x) = m_x$ ,  $COV(x) = \Sigma_x$  – SPD
  - $x, v$  are not correlated
- Seek  $\hat{x} = \Phi(z) = Az + b$ 
  - Linear, unbiased, min. variance estimate

# MINIMUM VARIANCE - CONTINUED

---

- Let  $\tilde{x} = x - \hat{x}$
- We seek to minimize mean squared error:

$$\begin{aligned} E[\tilde{\mathbf{x}}^T \tilde{\mathbf{x}}] &= E[(\mathbf{x} - \hat{\mathbf{x}})^T (\mathbf{x} - \hat{\mathbf{x}})] \\ &= E[\text{tr}[(\mathbf{x} - \hat{\mathbf{x}})^T (\mathbf{x} - \hat{\mathbf{x}})]] \\ &= E[\text{tr}[(\mathbf{x} - \hat{\mathbf{x}})(\mathbf{x} - \hat{\mathbf{x}})^T]] \\ &= \text{tr}[E(\mathbf{x} - \hat{\mathbf{x}})(\mathbf{x} - \hat{\mathbf{x}})^T] \\ &= \text{tr}(\mathbf{P}) \end{aligned}$$

where  $\text{COV}(\tilde{x}) = \mathbf{P}$

# CONDITION FOR UNBIASEDNESS

---

- $m = E(\hat{x}) = E(b + Az) = b + A \cdot E(Hx + v) = b + AHm$
- $b = (I - AH)m$
- $\hat{x} = b + Az = (I - AH)m + Az = m + A(z - Hm)$ 
  - Look at this structure – we saw it in Bayesian framework!
- $P = \text{COV}(\tilde{x}) = E[(x - \hat{x})(x - \hat{x})^T]$
- $x - \hat{x} = (x - m) - A(z - Hm)$
- $(x - \hat{x})^T(x - \hat{x}) = [(x - m) - A(z - Hm)][(x - m) - A(z - Hm)]^T$ 
$$= (x - m)(x - m)^T - (x - m)(z - Hm)^T A^T$$
$$- A(z - Hm)(x - m)^T + A(z - Hm)(z - Hm)^T A^T$$
- But  $z = Hx + v$ ,  $z - Hm = H(x - m) + v$

# EXPRESSION FOR THE VARIANCE

---

- $\therefore P = E(x - \hat{x})(x - \hat{x})^T$   
     $= E[(x - m)(x - m)^T] \rightarrow \Sigma_x$   
     $- E[(x - m)[(x - m)^T H^T + v^T]]A^T \rightarrow -\Sigma_x H^T A^T$   
     $- E[AH(x - m) + v][x - m]^T \rightarrow -AH\Sigma_x$   
     $+ A^T E[(H(x - m) + v)(H(x - m) + v)^T]A \rightarrow ADA^T$
- $P = \Sigma_x + ADA^T - AH\Sigma_x - \Sigma_x H^T A^T$ ,  $D = (H\Sigma_x H^T + \Sigma_v)$
- Thus  $P$  is a quadratic function of  $A|_{n \times m}$

# MINIMIZING THE TOTAL VARIANCE

---

- Minimize trace of  $P$  (total variance) w.r.t.  $A$
- $\text{tr}(P) = \sum_{i=1}^n P_{ii}$
- $P_{ii} = (\Sigma_x)_{ii} + A_{i*}DA_{i*}^T - A_{i*}b_{i*}^T - b_{i*}A_{i*}^T$ 
  - $b_{i*}$  =  $i$ th row of  $n \times m$  matrix  $\Sigma_x H^T$
- $P_{ii} = A_{i*}DA_{i*}^T - 2b_{i*}^T A_{i*} + (\Sigma_x)_{ii}$ 
  - $y = A_{i*}$   $i$ th row of  $A$ ,  $y^T = A_{i*}^T$
  - $b = b_{i*}^T$ ,  $b^T = b_{i*}$

# MINIMIZATION

---

- Minimize  $P_{ii}$  w.r.t  $y$  – a standard quadratic form
- $\nabla P_{ii} = 2Dy - 2b = 0$
- $\Rightarrow y = D^{-1}b$
- $\Rightarrow A_{i*}^T = D^{-1}b_{i*}^T$
- $[A_{1*}^T \ A_{2*}^T \ \dots \ A_{m*}^T] = D^{-1}[b_{1*}^T \ b_{2*}^T \ \dots \ b_{m*}^T]$

# OPTIMAL P

---

- $A^T = D^{-1}H\Sigma_x$
- $A = \Sigma_x H^T D^{-1}$   
 $= \Sigma_x H^T [H\Sigma_x H^T + \Sigma_v]^{-1}$
- $\therefore \hat{X} = m + \Sigma_x H^T [H\Sigma_x H^T + \Sigma_v]^{-1} [z - Hm]$
- Substituting A in P
- $\Rightarrow P = \Sigma_x - \Sigma_x H^T [H\Sigma_x H^T + \Sigma_v]^{-1} H \Sigma_x$

Subtracted

# RELATION BETWEEN BAYES L.S. SOLUTION AND LINEAR MIN. VARIANCE SOLUTION - DUALITY

---

- Bayesian – state space
  - $\hat{x}_{MS} = \Sigma_e [H^T \Sigma_v^{-1} z + \Sigma_e^{-1} m_x] \rightarrow (16.2.26)$
  - $\Sigma_e = [H^T \Sigma_e^{-1} H + \Sigma_e]^{-1} = \text{COV}(\hat{x}_{MS}) \rightarrow (16.2.25)$
  - State-space, used for  $n < m$
- L.M.V. – observation space
  - $\hat{x} = m + \Sigma_x H^T [H \Sigma_x H^T + \Sigma_v]^{-1} [z - Hm] \rightarrow (17.1.15)$
  - $P = \Sigma_x - \Sigma_x H^T [H \Sigma_x H^T + \Sigma_v]^{-1} H \Sigma_x \rightarrow (17.1.11)$
  - Observation space, used for  $m < n$
- They are the same!

# BRIDGE: SHERMAN-MORRISON-WOODBURY LEMMA IN MATRIX THEORY (APPENDIX B)

---

- LMV

- Recall:  $D = (H\Sigma_x H^T + \Sigma_v)$

- $D^{-1} = (H\Sigma_x H^T + \Sigma_v)^{-1}$   
 $= \Sigma_v^{-1} - \Sigma_v^{-1} H [H^T \Sigma_v^{-1} H + \Sigma_x^{-1}]^{-1} H^T \Sigma_v^{-1}$

- Multiply both side by  $\Sigma_x H^T$

$$\Sigma_x H^T [H\Sigma_v H^T + \Sigma_v]^{-1}$$

$$= \Sigma_x H^T \Sigma_v^{-1} - \Sigma_x H^T \Sigma_v^{-1} H [H^T \Sigma_v^{-1} H + \Sigma_x^{-1}]^{-1} H^T \Sigma_v^{-1}$$

$$= \{\Sigma_x - \Sigma_x H^T \Sigma_v^{-1} H [H^T \Sigma_v^{-1} H + \Sigma_v^{-1}]^{-1}\} H^T \Sigma_v^{-1}$$

$$= \{\Sigma_x [H^T \Sigma_v^{-1} H + \Sigma_x^{-1}] - \Sigma_x H^T \Sigma_v^{-1} H\} (H^T \Sigma_v^{-1} H + \Sigma_x^{-1})^{-1} H^T \Sigma_v^{-1}$$

$$= I \cdot (H^T \Sigma_v^{-1} H + \Sigma_x^{-1})^{-1} H^T \Sigma_v^{-1}$$

# SHERMAN-MORRISON-WOODBURY CONTINUED

---

- Now, substitute in (17.1.15)

$$\begin{aligned}\hat{x} &= m + \Sigma_x H^T [H \Sigma_x H^T + \Sigma_v]^{-1} (z - Hm) \\ &= m + (H^T \Sigma_v^{-1} H + \Sigma_x^{-1})^{-1} H^T \Sigma_v^{-1} (z - Hm) \\ &= (H^T \Sigma_v^{-1} H + \Sigma_x^{-1})^{-1} H^T \Sigma_v^{-1} z \\ &\quad + \{I - (H^T \Sigma_v^{-1} H + \Sigma_x^{-1})^{-1} H^T \Sigma_v^{-1} H\} m\end{aligned}$$

- Consider the second term:

$$\begin{aligned}\{I - (H^T \Sigma_v^{-1} H + \Sigma_x^{-1})^{-1} H^T \Sigma_v^{-1} H\} m \\ &= (H^T \Sigma_v^{-1} H + \Sigma_x^{-1})^{-1} [(H^T \Sigma_v^{-1} H + \Sigma_x^{-1}) - H^T \Sigma_v^{-1} H] m \\ &= (H^T \Sigma_v^{-1} H + \Sigma_x^{-1})^{-1} [\Sigma_x^{-1} m]\end{aligned}$$

- Combining

$$\hat{x} = (H^T \Sigma_v^{-1} H + \Sigma_x^{-1})^{-1} [\Sigma_x^{-1} m + H^T \Sigma_v^{-1} z]$$

# KALMAN FILTERS - STATIC CASE

---

- $x \in \mathbb{R}^n$  – unknown, constant
- $x^-$  is an unbiased estimate of  $x$  if no observation.
- $E(x^-) = x$
- $(x^-, \Sigma_-)$  – prior information
  - $z = Hx + v$ ,  $E(v) = 0$ ,  $\text{COV}(v) = \Sigma_v$
  - Usual conditions on  $v$
- Linear Min. Variance Approach
  - $x^+ = Lx^- + Kz$  ( $x^+$ : posterior)
  - Find  $L$ ,  $K$  such that  $x^+$  is unbiased and has minimum variance

# STATIC CASE - CONTINUED

---

- (a) Unbiasedness:

- $x^+ = Lx^- + Kz$

- $x = E(x^+)$

- $= E[Lx^- + Kz]$

- $= E[Lx^- + K(Hx + v)]$

- $= LE(x^-) + KHx + \cancel{KE(v)}$

- $= Lx + KHx = (L + KH)x$

- $\therefore L + KH = I$  or  $L = I - KH$

- $\therefore x^+ = Lx^- + Kz$

- $= (I - KH)x^- + Kz$  ← structure of the unbiased estimate

- $= x^- + K[z - Hx^-]$

# STATIC CASE - CONTINUED

---

- We now need to compute the total variance of  $x^+$
- $\text{var}(x^+) = E[(x^+ - x)^T(x^+ - x)]$ 
$$= E[\text{tr}[(x^+ - x)^T(x^+ - x)]]$$
$$= E[\text{tr}[(x^+ - x)(x^+ - x)^T]]$$
$$= \text{tr}(\Sigma^+)$$
- Recall:
  - $x^+ = (I - KH)x^- + Kz$ 
$$= (I - KH)x^- + KHx + Kv$$
  - $\therefore x^+ - x = (I - KH)x^- + KHx - x + Kv$ 
$$= (I - KH)(x^- - x) + Kv$$

# STATIC CASE - CONTINUED

---

- $\therefore \Sigma^+ = E[(I - KH)(x^- - x) + Kv] [(I - KH)(x^- - x) + Kv]^T$ 
$$= (I - KH)E[(x^- - x)(x^- - x)^T](I - KH)^T + KE(vv^T)K^T$$
$$= (I - KH)\Sigma_-(I - KH)^T + K\Sigma_v K^T$$
$$= \Sigma_- + KDK^T - KH\Sigma_- - \Sigma_-H^TK^T$$
$$D = (H\Sigma_-H^T + \Sigma_v)$$
- Choose  $K$  to minimize  $\text{tr}(\Sigma^+)$
- Similar to the problem we just solved.
  - $\Rightarrow K = \Sigma_-H^TD^{-1}$ 
$$= \Sigma_-H^T[H\Sigma_-H^T + \Sigma_v]^{-1}$$

Kalman gain

# STATIC CASE - CONTINUED

---

- $\therefore x^+ = x^- + \Sigma_- H^T [H \Sigma_- H^T + \Sigma_v]^{-1} [z - H x^-]$   
 $\Sigma^+ = \Sigma_- - \Sigma_- H^T [H \Sigma_- H^T + \Sigma_v]^{-1} H \Sigma_-$

# EXERCISES

---

1.  $\Sigma_+$  does not depend on observations and hence can be precomputed – Verify this claim

2. Reformulate as 3-D Var

$$(x^-, \Sigma_-) \text{ and } (z, \Sigma_v) \quad z = Hx + v$$

$$f(x) = \frac{1}{2}(z - Hx)^T \Sigma_v^{-1} (z - Hx) + \frac{1}{2}(x^- - x)^T \Sigma_-^{-1} (x^- - x)$$

Min.  $f(x)$  w.r. to  $x$  and find the solution

# REFERENCE

---

- A. P. Sage and J. L. Melsa (1971) Estimation Theory and its application to communications and Control, *McGraw Hill*
- Also refer to chapter 17 in LLD (2006)